substitutions for directions

theories/DirectedDirectioning.v
@@ -10,6 +10,7 @@ Set Primitive Projections.
 
 Reserved Notation "[ δ |- t ◃ d ]" (at level 0, δ, d, t at level 50, only parsing).
 Reserved Notation "[ δ |- t ▹ d ]" (at level 0, δ, d, t at level 50, only parsing).
+Reserved Notation "[ δ |-s σ ◃ γ ]" (at level 0, δ, γ, σ at level 50, only parsing).
 
 
 Inductive DirInfer (δ : list direction) : direction -> term -> Type :=
@@ -154,11 +155,11 @@ Definition dir_wk {Γ Δ} (ρ : Γ ≤ Δ) (δ γ : list direction) :=
   forall n d, List.nth_error γ n = Some d ->
   ∑ d', (List.nth_error δ (ρ n) = Some d') × dir_leq d' d.
 
-Lemma dir_wk_up_discr {Γ Δ A γ δ} (ρ : Γ ≤ Δ) : dir_wk ρ δ γ -> dir_wk (wk_up A ρ) (Discr :: δ) (Discr :: γ).
+Lemma dir_wk_up {Γ Δ A γ δ d} (ρ : Γ ≤ Δ) : dir_wk ρ δ γ -> dir_wk (wk_up A ρ) (d :: δ) (d :: γ).
 Proof.
-  intros hρ [|n] d ; cbn.
-  - intros [= <-]; exists Discr; now split.
-  - intros [d' [-> ]]%hρ; exists d'; now split.
+  intros hρ [|n] d' ; cbn.
+  - intros [= <-]; exists d; now split.
+  - intros [d'' [-> ]]%hρ; exists d''; now split.
 Qed.
 
 
@@ -183,7 +184,7 @@ Proof.
     tea.
   - intros * dirA ihA dirB ihB ? * hρ.
     destruct (ihA _ _ _ _ hρ) as [d1 [dirA' leq1]].
-    destruct (ihB _ _ _ _ (dir_wk_up_discr _ hρ (A:=A))) as [d2 [dirB' leq2]].
+    destruct (ihB _ _ _ _ (dir_wk_up _ hρ (A:=A))) as [d2 [dirB' leq2]].
     assert (dir_op d1 ⪯ d'').
     by (etransitivity; try apply dir_op_mon; tea; now eapply MaxDirProp.upper_bound1).
     assert (d2 ⪯ d'').
@@ -193,7 +194,7 @@ Proof.
     1: now econstructor.
     eapply MaxDirProp.max_least; tea.
   - intros * dirt iht ? * hρ.
-    destruct (iht _ _ _ _ (dir_wk_up_discr _ hρ (A:=A))) as [d1 [dirt' leq1]].
+    destruct (iht _ _ _ _ (dir_wk_up _ hρ (A:=A))) as [d1 [dirt' leq1]].
     eexists; split; tea.
     now econstructor.
   - intros * dirf ihf dira iha ? * hρ.
@@ -203,17 +204,111 @@ Proof.
     now apply iha.
 Qed.
 
-Lemma dir_subst_Discr {δ d B a} :
-  [ δ |- a ◃ Discr ] -> [ cons Discr δ |- B ◃ d ] -> [ δ |- B[a..] ◃ d ].
-Proof.
-Admitted.
 
-Inductive dir_ctx : context -> list direction -> list direction -> Type :=
-| dirNil : dir_ctx nil nil nil
-| dirCons {Γ δ δty A d dA} : DirCheck δ dA A -> dir_ctx Γ δ δty -> dir_ctx (cons A Γ) (cons d δ) (cons dA δty).
+(* Inductive DirSubst (δ: list direction) : list direction -> (nat -> term) -> Type:= *)
+(* | dirSEmpty {σ} : [ δ |-s σ ◃ nil ] *)
+(* | dirSCons {σ γ d} : *)
+(*   [ δ |-s ↑ >> σ ◃ γ ] -> *)
+(*   [ δ |- σ var_zero ◃ d ] -> *)
+(*   [ δ |-s σ ◃ cons d γ ] *)
+(* where "[ δ '|-s' σ ◃ γ ]" := (DirSubst δ γ σ). *)
+
+
+Definition DirSubst (δ γ : list direction) (σ: nat -> term) :=
+  forall n d, List.nth_error γ n = Some d -> [ δ |- σ n ◃ d ].
+Notation "[ δ '|-s' σ ◃ γ ]" := (DirSubst δ γ σ).
+
+
+Lemma dir_subst_up {δ γ d σ} :
+  [ δ |-s σ ◃ γ ] ->
+  [ cons d δ |-s σ⟨↑⟩ ◃ γ ].
+Proof.
+  intros H n d' eq.
+  change [(d :: δ) |- (σ n)⟨↑⟩ ◃ d'].
+  eapply (Datatypes.snd (dir_infer_check_ren _)).
+  1: now apply H.
+  exact dir_ren1.
+Qed.
+
+Lemma dir_subst_up_term_term {δ γ d σ} :
+  [ δ |-s σ ◃ γ ] -> [ (d :: δ) |-s up_term_term σ ◃ (d :: γ) ].
+Proof.
+  intros H [|n] d'.
+  - cbn. intros [=->].
+    econstructor. 1: constructor; reflexivity. reflexivity.
+  - cbn. intros eq. now eapply dir_subst_up.
+Qed.
+
+Lemma dir_id_subst {δ} :
+  [δ |-s tRel ◃ δ].
+Proof.
+  intros n d eq. econstructor.
+  1: now constructor.  reflexivity.
+Qed.
+
+Lemma dir_subst_var {δ γ n d σ} :
+  List.nth_error γ n = Some d -> [δ |-s σ ◃ γ] -> [δ |- (tRel n)[σ] ◃ d].
+Proof.
+  intros nth H.
+  now apply H.
+Qed.
+
+Lemma dir_infer_check_subst γ
+  (Pinfer:= fun γ d t _ => forall δ σ, [ δ |-s σ ◃ γ ] -> ∑ d', [δ |- t[σ] ▹ d'] * dir_leq d' d)
+  (Pcheck := fun γ d t _ => forall δ σ, [ δ |-s σ ◃ γ ] -> [δ |- t[σ] ◃ d])
+:
+  (forall d t (der : [γ |- t ▹ d]), Pinfer γ d t der)
+  * (forall d t (der : [γ |- t ◃ d]), Pcheck γ d t der).
+Proof.
+  apply DirInferCheck_rect.
+  all: unfold Pinfer, Pcheck.
+  - econstructor; split; constructor.
+  - intros.
+    unshelve epose (Y := dir_subst_var _ _). 6,7: tea. inversion Y; subst.
+    eexists; split; tea.
+  - intros * dirA ihA dirB ihB ? * hσ.
+    destruct (ihA _ _ hσ) as [d1 [dirA' leq1]].
+    destruct (ihB _ _ (dir_subst_up_term_term hσ)) as [d2 [dirB' leq2]].
+    assert (dir_op d1 ⪯ d'').
+    by (etransitivity; try apply dir_op_mon; tea; now eapply MaxDirProp.upper_bound1).
+    assert (d2 ⪯ d'').
+    by (etransitivity; tea; now eapply MaxDirProp.upper_bound2).
+    unshelve epose proof (MaxDirProp.max_exists (dir_op d1) d2 d'' _ _) as [d3]; tea.
+    exists d3; split.
+    1: now econstructor.
+    eapply MaxDirProp.max_least; tea.
+  - intros * dirt iht ? * hσ.
+    destruct (iht _ _ (dir_subst_up_term_term hσ)) as [d1 [dirt' leq1]].
+    eexists; split; tea.
+    now econstructor.
+  - intros * dirf ihf dira iha ? * hσ.
+    destruct (ihf _ _ hσ) as [d1 [dirf' leq1]].
+    eexists; split; tea.
+    constructor; tea.
+    now apply iha.
+  - intros * ? ih **; edestruct ih as [? []]; tea; econstructor; tea.
+    now etransitivity.
+Qed.
+
+Lemma dir_subst1 {δ d d' B a} :
+  [ δ |- a ◃ d' ] -> [ cons d' δ |- B ◃ d ] -> [ δ |- B[a..] ◃ d ].
+Proof.
+  intros.
+  eapply dir_infer_check_subst; tea.
+  intros [|n] d''.
+  - cbn. now intros [=->]. (* TODO: lemma for subst cons *)
+  - intros eq. inversion eq. cbv.
+    econstructor.
+    1: now constructor.
+    reflexivity.
+Qed.
+
+Inductive DirCtx : context -> list direction -> list direction -> Type :=
+| dirNil : DirCtx nil nil nil
+| dirCons {Γ δ δty A d dA} : DirCheck δ dA A -> DirCtx Γ δ δty -> DirCtx (cons A Γ) (cons d δ) (cons dA δty).
 
 Lemma dir_ctx_nth_ty {Γ δ δT} :
-  dir_ctx Γ δ δT ->
+  DirCtx Γ δ δT ->
   forall n T dT, in_ctx Γ n T ->
   List.nth_error δT n = Some dT ->
   [δ |- T ◃ dT].
